rename hash table impl as sharedexclusive-linearhandoverhand in prep for alternative impls; factor out common stuff

concurrency/disciplined/sharedexclusive-linearhandoverhand/ShardedHashTable.i.dfy
@@ -1,82 +1,10 @@
-include "../../lib/Lang/NativeTypes.s.dfy"
-include "../../lib/Base/Option.s.dfy"
-include "ConcurrencyModel.s.dfy"
-include "AppSpec.s.dfy"
-
-module Limits {
-  import opened NativeTypes
-
-  function FixedSize() : (n: nat)
-    ensures n > 1
-
-  function Capacity() : (n: nat)
-  {
-    FixedSize() - 1
-  }
-
-  function method FixedSizeImpl() : (n: uint32)
-    ensures n as int == FixedSize()
-
-  function method CapacityImpl(): (s: uint32)
-    ensures s as nat == Capacity()
-}
-
-// Build up the insert_capacity monoid first so we can talk about it separately
-// in the CapacityAllocator impl, and not have to cart around an entire ShardedHashTable.
-module Count refines PartialCommutativeMonoid {
-  import opened Limits
-
-  datatype Variables = Variables(value: nat)
-
-  function unit() : Variables { Variables(0) }
-
-  function add(x: Variables, y: Variables) : Variables {
-    Variables(x.value + y.value)
-  }
-
-  lemma add_unit(x: Variables)
-  ensures add(x, unit()) == x
-  {
-  }
-
-  lemma commutative(x: Variables, y: Variables)
-  ensures add(x, y) == add(y, x)
-  {
-  }
-
-  lemma associative(x: Variables, y: Variables, z: Variables)
-  ensures add(x, add(y, z)) == add(add(x, y), z)
-  {
-  }
-
-  predicate Inv(s: Variables)
-  {
-    s.value <= Capacity()
-  }
-
-  predicate Valid(s: Variables)
-  {
-    exists t :: Inv(add(s, t))
-  }
-
-  function {:opaque} GetRemainder(s: Variables): (t: Variables)
-    requires Valid(s)
-    ensures Inv(add(s, t))
-  {
-    // reveal Valid();
-    var t :| Inv(add(s, t));
-    t
-  }
-
-  lemma valid_monotonic(x: Variables, y: Variables)
-  //requires Valid(add(x, y))
-  ensures Valid(x)
-  {
-  }
-}
+include "../../../lib/Lang/NativeTypes.s.dfy"
+include "../../../lib/Base/Option.s.dfy"
+include "../common/ConcurrencyModel.s.dfy"
+include "../common/AppSpec.s.dfy"
+include "../common/CountMonoid.i.dfy"
 
 // TODO(jonh): refactor ShardedHashTable into this module chain:
-
 module ShardedSMTransitions  {
   // Extracted from 
 }
