concurrency/disciplined/common/Limits.i.dfy
@@ -1,0 +1,23 @@
+include "../../../lib/Lang/NativeTypes.s.dfy"
+include "../../../lib/Base/Option.s.dfy"
+include "ConcurrencyModel.s.dfy"
+include "AppSpec.s.dfy"
+
+module Limits {
+  import opened NativeTypes
+
+  function FixedSize() : (n: nat)
+    ensures n > 1
+
+  function Capacity() : (n: nat)
+  {
+    FixedSize() - 1
+  }
+
+  function method FixedSizeImpl() : (n: uint32)
+    ensures n as int == FixedSize()
+
+  function method CapacityImpl(): (s: uint32)
+    ensures s as nat == Capacity()
+}
+
